\documentclass[a4paper, 12pt]{article}
\usepackage[a4paper,top=1.5cm, bottom=1.5cm, left=1cm, right=1cm]{geometry}
\usepackage[utf8]{inputenc}
\usepackage{mathtext}
\usepackage{amsmath}
\usepackage{amssymb}
\usepackage{amsfonts}
\usepackage{textcomp}
\usepackage[english, russian]{babel}
\usepackage{indentfirst}
\usepackage{fixltx2e}
\usepackage{longtable}
\usepackage{graphicx}
\usepackage{tabto}
\graphicspath{{pictures/}}
\DeclareGraphicsExtensions{.pdf,.png,.jpg}
\usepackage{natbib}
\usepackage{mathrsfs}
\usepackage[europeanresistors, americaninductors]{circuitikz}
\renewcommand{\t}[1]{\hspace{#1mm}}
\newcommand{\n}{\par{}}
\renewcommand{\a}{\bigcap{}}
\renewcommand{\u}{\bigcup{}}
\newcommand{\png}[1]{\includegraphics[width=200pt]{~/Documents/#1.png}\n}
\renewcommand{\d}{$}
\renewcommand{\i}{^{-1}}
\renewcommand{\d}{$}
\newcommand{\dand}{$\land$}
\newcommand{\dor}{$\lor$}
\newcommand{\dno}[1]{$\overline{#1}$}
\newcommand{\dnot}{$\neg$}
\newcommand{\ans}{Ответ: }




\title{АЛКТГ дз 2}
\author{Татаринов Георгий}
\date{\today}

\begin{document}
	\maketitle
	\section*{Задание 1}
		а) $a_k = k$. Тогда производящая функция равна:

		$\sum\limits_{k = 0}^{\infty} (k*x^k)$

		$\dfrac{1}{1 - x}=1 + x + x^2 ... $

		$(\dfrac{1}{1 - x})'= 1 + 2x + 3x^2 + ... = \sum\limits_{k = 0}^{\infty} kx^{k-1}$

		$(\dfrac{1}{1 - x})' * x = (1 + 2x + 3x^2 + ...) * x = \sum\limits_{k = 0}^{\infty} kx^k$

		Ответ: $\dfrac{x}{(1 - x)^2}$ - производящая функция последовательности $a_k$

		б) $a_k = \dfrac{1}{k!}$. Тогда производящая функция равна:

		$\sum\limits_{k = 0}^{\infty} \dfrac{x^k}{k!}$

		$e^x=\sum\limits_{k = 0}^{\infty} \dfrac{x^k}{k!}$

		Ответ: $e^x$ - производящая функция последовательности $a_k$
	\section*{Задание 2}
	\section*{Задание 3}
	\section*{Задание 4}
		Пусть f(x)=$\sum\limits_{k=0}^{n}C_n^k*x^k=(1+x)^n$

		f '(x)=$\sum\limits_{k=0}^{n}C_n^k*k*x^{k-1}=n*(1+x)^{n-1}$

		f ''(x)=$\sum\limits_{k=0}^{n}C_n^k*k*(k-1)*x^{k-2}=n*(n-1)*(1+x)^{n-2}$

		f ''(x)=$\sum\limits_{k=2}^{n}C_n^k*k*(k-1)*x^{k-2}=n*(n-1)*(1+x)^{n-2}$

		При x=1

		$\sum\limits_{k=2}^{n}C_n^k*k*(k-1)=n*(n-1)*2^{n-2}$
	\section*{Задание 5}
		$g(x)=\sum\limits_{k=0}^{\infty}(x^k*s_k)$

		$x*g(x)=\sum\limits_{k=0}^{\infty}(x^{k+1}*s_k)$

		$x*g(x)=\sum\limits_{k=1}^{\infty}(x^{k}*s_{k-1})$

		$x*g(x)-g(x)=\sum\limits_{k=1}^{\infty}(x^k*s_{k-1}-x^k*s_k)+s_0$

		$x*g(x)-g(x)=\sum\limits_{k=1}^{\infty}(x^k*a_{k})+s_0$

		$x*g(x)-g(x)=\sum\limits_{k=0}^{\infty}(x^k*a_{k})$

		Ответ: $x*g(x)-g(x)$
	\section*{Задание 6}
		При x$\neq$ 0

		$\lim\limits_{n->\infty}\sum\limits_{i=0}^{n}\dfrac{x^i}{i+1}=1/x*\lim\limits_{n->\infty}\sum\limits_{i=0}^{n}\dfrac{x^{i+1}}{i+1}=1/x*\lim\limits_{n->\infty}\sum\limits_{i=1}^{n}\dfrac{x^i}{i}=-\dfrac{ln(1-x)}{x}$

		При x=0

		$\lim\limits_{n->\infty}\sum\limits_{i=0}^{n}\dfrac{x^i}{i+1}=1$

		Ответ: $-\dfrac{ln(1-x)}{x}$ при x$\neq$0 и 1 при x=0
\end{document}
